Progress on LTS sim

ChoiceTrees/CTree.v
@@ -97,94 +97,87 @@ Proof.
   lia.
 Qed.
 
+Lemma ole_or_olt x y : ole x y ∨ olt y x.
+Proof.
+  unfold ole, olt.
+  destruct x as [x|], y as [y|]; simpl; eauto.
+  destruct (PeanoNat.Nat.eq_dec x y); subst; eauto.
+  lia.
+Qed.
+
 Lemma ole_top x : ole x None.
 Proof. destruct x; cbv; eauto. Qed.
 
 (* from FreeSim (Stuttering for Free) *)
 (* infinite silent steps should be equivalent only to infinite silent steps *)
-Inductive RefineF {R1 R2 E r sim}
+Inductive SimF {R1 R2 E r sim}
   : option nat → option nat → CTree' E R1 → CTree' E R2 → Prop :=
 | refine_prog p1 p2 t1 t2 p1' p2'
   (* only rule that strictly decrements the progress indices*)
   (LT1 : p1' ≺ p1) (LT2 : p2' ≺ p2)
   (SIM : sim p1' p2' t1 t2)
-: RefineF p1 p2 t1 t2
+: SimF p1 p2 t1 t2
 | refine_ret p1 p2 x y
   (RET : r x y : Prop)
-: RefineF p1 p2 (Ret x) (Ret y)
+: SimF p1 p2 (Ret x) (Ret y)
 | refine_vis p1 p2 p1' p2' {A} (e : E A) k1 k2
   (CONT : ∀ a, sim p1' p2' (obs_ctree (k1 a)) (obs_ctree (k2 a)))
-: RefineF p1 p2 (Vis e k1) (Vis e k2)
+: SimF p1 p2 (Vis e k1) (Vis e k2)
 | refine_zero p1 p2 t2
-: RefineF p1 p2 Zero t2
+: SimF p1 p2 Zero t2
 | refine_choiceL p1 p2 p1' t2 k
-  (CHOICE : ∀ c, RefineF p1' p2 (obs_ctree (k c)) t2)
-: RefineF p1 p2 (Choice k) t2
+  (CHOICE : ∀ c, SimF p1' p2 (obs_ctree (k c)) t2)
+: SimF p1 p2 (Choice k) t2
 | refine_choiceR p1 p2 p2' t1 k
-  c (CHOICE : RefineF p1 p2' t1 (obs_ctree (k c)))
-: RefineF p1 p2 t1 (Choice k)
+  c (CHOICE : SimF p1 p2' t1 (obs_ctree (k c)))
+: SimF p1 p2 t1 (Choice k)
 .
 
-Arguments RefineF {_ _ _} _ _.
+Arguments SimF {_ _ _} _ _.
 
 Section IND.
   Context {R1 R2 E} (r : R1 → R2 → Prop) (sim : option nat → option nat → CTree' E R1 → CTree' E R2 → Prop).
-  Context (P : ∀ p1 p2 t1 t2, RefineF r sim p1 p2 t1 t2 → Prop).
+  Context (P : ∀ p1 p2 t1 t2, SimF r sim p1 p2 t1 t2 → Prop).
   Context (Pprog : ∀ p1 p2 t1 t2 p1' p2' LT1 LT2 SIM, P _ _ _ _ (refine_prog p1 p2 t1 t2 p1' p2' LT1 LT2 SIM))
           (Pret : ∀ p1 p2 x y RET, P _ _ _ _ (refine_ret p1 p2 x y RET))
           (Pvis : ∀ p1 p2 p1' p2' A (e : E A) k1 k2 CONT, P _ _ _ _ (refine_vis p1 p2 p1' p2' e k1 k2 CONT))
           (Pzero : ∀ p1 p2 t2, P _ _ _ _ (refine_zero p1 p2 t2))
           (PL : ∀ p1 p2 p1' t2 k CHOICE (IHk : ∀ c, P _ _ _ _ (CHOICE c)), P _ _ _ _ (refine_choiceL p1 p2 p1' t2 k CHOICE))
           (PR : ∀ p1 p2 p2' t1 k c CHOICE (IHk : P _ _ _ _ CHOICE), P _ _ _ _ (refine_choiceR p1 p2 p2' t1 k c CHOICE)).
-  Fixpoint RefineF_ind p1 p2 t1 t2 pf : P p1 p2 t1 t2 pf.
+  Fixpoint SimF_ind p1 p2 t1 t2 pf : P p1 p2 t1 t2 pf.
   Proof.
     destruct pf.
     - apply Pprog.
     - apply Pret.
     - apply Pvis.
     - apply Pzero.
-    - apply PL. intros. apply RefineF_ind.
-    - apply PR. intros. apply RefineF_ind.
-  Qed.
-End IND.
-
-(* branch t t' : t has less choice than t' *)
-Inductive branch {R E} : CTree' E R → CTree' E R → Prop :=
-| branch_refl t
-: branch t t
-| branch_zero t
-: branch Zero t
-| branch_choice k1 k2
-  (CHOICE : ∀ c1, {c2 | branch (obs_ctree (k1 c1)) (obs_ctree (k2 c2))})
-: branch (Choice k1) (Choice k2)
-.
-
-Section IND.
-  Context {R : Type} {E : Type → Type}.
-  Context (P : ∀ (t1 t2 : CTree' E R), branch t1 t2 → Prop).
-  Context (Prefl : ∀ t, P _ _ (branch_refl t))
-          (Pzero : ∀ t, P _ _ (branch_zero t))
-          (Pchoice : ∀ k1 k2 CHOICE
-            (IHk : ∀ c1, P _ _ (proj2_sig (CHOICE c1))),
-            P _ _ (branch_choice k1 k2 CHOICE)).
-  Fixpoint branch_ind t1 t2 pf : P t1 t2 pf.
-  Proof.
-    destruct pf.
-    - apply Prefl.
-    - apply Pzero.
-    - apply Pchoice. intros. apply branch_ind.
+    - apply PL. intros. apply SimF_ind.
+    - apply PR. intros. apply SimF_ind.
   Qed.
 End IND.
 
 Definition BisimF {R1 R2 E} (φ : R1 → R2 → Prop) sim p1 p2 t1 t2 :=
-  RefineF (E := E) φ sim p1 p2 t1 t2 ∧
-  RefineF
+  SimF (E := E) φ sim p1 p2 t1 t2 ∧
+  SimF
     (fun r1 r2 => φ r2 r1)
     (fun p1 p2 t1 t2 => sim p2 p1 t2 t1)
     p2 p1 t2 t1
 .
 
-Lemma RefineF_monotone R1 R2 E r : monotone4 (@RefineF R1 R2 E r).
+(* divergence predicate *)
+Variant divF {E R sim} : CTree' E R → Prop :=
+| div_intro k c (SIM : sim (obs_ctree (k c)) : Prop)
+: divF (Choice k)
+.
+
+Arguments divF {_ _} _ _.
+
+Lemma divF_monotone {E R} : monotone1 (@divF E R).
+Proof. repeat intro. destruct IN. econstructor; eauto. Qed.
+
+Hint Resolve divF_monotone : paco.
+
+Lemma SimF_monotone R1 R2 E r : monotone4 (@SimF R1 R2 E r).
 Proof.
   repeat intro. revert r' LE. induction IN; intros.
   - econstructor 1; eauto.
@@ -195,45 +188,47 @@ Proof.
   - econstructor 6; eauto.
 Qed.
 
-Hint Resolve RefineF_monotone : paco.
+Hint Resolve SimF_monotone : paco.
 
 Lemma BisimF_monotone R1 R2 E φ : monotone4 (@BisimF R1 R2 E φ).
 Proof.
   repeat intro.
   destruct IN as (IN & IN').
-  split; eapply RefineF_monotone; eauto.
+  split; eapply SimF_monotone; eauto.
 Qed.
 
 Hint Resolve BisimF_monotone : paco.
 
-Definition Refine {R1 R2 E} r := paco4 (@RefineF R1 R2 E r) bot4.
+Definition Sim {R1 R2 E} r := paco4 (@SimF R1 R2 E r) bot4.
 
 Definition Bisim {R1 R2 E} r := paco4 (@BisimF R1 R2 E r) bot4.
 
-Lemma Refine_postfix {R1 R2 E} (φ : R1 → R2 → Prop) :
-  Refine (E := E) φ <4= RefineF φ (Refine φ).
+Definition div {E R} := paco1 (@divF E R) bot1.
+
+Lemma Sim_postfix {R1 R2 E} (φ : R1 → R2 → Prop) :
+  Sim (E := E) φ <4= SimF φ (Sim φ).
 Proof.
   repeat intro. punfold PR.
-  eapply RefineF_monotone; eauto.
+  eapply SimF_monotone; eauto.
   intros. pclearbot. auto.
 Qed.
 
 Lemma Bisim_postfix {R1 R2 E} (φ : R1 → R2 → Prop) :
-  Bisim (E := E) φ <4= RefineF φ (Bisim φ).
+  Bisim (E := E) φ <4= SimF φ (Bisim φ).
 Proof.
   repeat intro.
   punfold PR. destruct PR.
-  eapply RefineF_monotone; eauto.
+  eapply SimF_monotone; eauto.
   intros. pclearbot. auto.
 Qed.
 
 Lemma Bisim_postfix_flipped {R1 R2 E} (φ : R1 → R2 → Prop) :
   (fun p1 p2 t1 t2 => Bisim (E := E) φ p2 p1 t2 t1) <4=
-  RefineF (fun r1 r2 => φ r2 r1) (fun p1 p2 t1 t2 => Bisim φ p2 p1 t2 t1).
+  SimF (fun r1 r2 => φ r2 r1) (fun p1 p2 t1 t2 => Bisim φ p2 p1 t2 t1).
 Proof.
   repeat intro.
   punfold PR. destruct PR.
-  eapply RefineF_monotone; eauto.
+  eapply SimF_monotone; eauto.
   intros. pclearbot. auto.
 Qed.
 
@@ -257,10 +252,10 @@ Definition comp4 {E R1 R2 R3}
   ∃ p12 p21 t2, sim12 p11 p12 t1 t2 ∧ sim23 p21 p22 t2 t3
 .
 
-Lemma RefineF_index_mono {R1 R2 E} φ (sim : _ → _ → _ → _ → Prop) :
-  ∀ p1 p2 (t1 : CTree' E R1) (t2 : CTree' E R2) (REFINE : RefineF φ sim p1 p2 t1 t2)
+Lemma SimF_index_mono {R1 R2 E} φ (sim : _ → _ → _ → _ → Prop) :
+  ∀ p1 p2 (t1 : CTree' E R1) (t2 : CTree' E R2) (REFINE : SimF φ sim p1 p2 t1 t2)
     p1' p2' (LE1 : p1 ≼ p1') (LE2 : p2 ≼ p2'),
-    RefineF φ sim p1' p2' t1 t2.
+    SimF φ sim p1' p2' t1 t2.
 Proof.
   do 4 intro. induction 1.
   - intros p1'' p2'' ? ?.
@@ -276,14 +271,14 @@ Proof.
     intros. eapply IHREFINE; eauto. right; auto.
 Qed.
 
-Lemma RefineF_contR {R1 R2 E φ sim} (POSTFIX : sim <4= RefineF φ sim) :
+Lemma SimF_contR {R1 R2 E φ sim} (POSTFIX : sim <4= SimF φ sim) :
   ∀ p1 p2 (t1 : CTree' E R1) (t2' : CTree' E R2)
     (* if t1 refines t2', *)
-    (REFINE : RefineF φ sim p1 p2 t1 t2')
+    (REFINE : SimF φ sim p1 p2 t1 t2')
     (* for any t2 that may continue as t2', *)
     t2 k2 (OBS : t2 = Choice k2) c2 (BR : t2' = obs_ctree (k2 c2))
     (* t1 must refine t2 *)
-    p1' p2', RefineF φ sim p1' p2' t1 t2.
+    p1' p2', SimF φ sim p1' p2' t1 t2.
 Proof.
   induction p1 using (well_founded_induction olt_wf).
   rename H into IHp1.
@@ -301,10 +296,10 @@ Proof.
   Unshelve. all: exact None.
 Qed.
 
-Lemma RefineF_index_insensitive {R1 R2 E φ sim} (POSTFIX : sim <4= RefineF φ sim) :
-  ∀ p1 p2 (t1 : CTree' E R1) (t2 : CTree' E R2) (REFINE : RefineF φ sim p1 p2 t1 t2)
+Lemma SimF_index_insensitive {R1 R2 E φ sim} (POSTFIX : sim <4= SimF φ sim) :
+  ∀ p1 p2 (t1 : CTree' E R1) (t2 : CTree' E R2) (REFINE : SimF φ sim p1 p2 t1 t2)
     p1' p2',
-    RefineF φ sim p1' p2' t1 t2.
+    SimF φ sim p1' p2' t1 t2.
 Proof.
   do 2 intro. revert p1.
   induction p2 using (well_founded_induction olt_wf).
@@ -316,7 +311,7 @@ Proof.
   - intros. econstructor 3; eauto.
   - intros. econstructor 4; eauto.
   - intros. econstructor 5; eauto.
-  - intros. eapply RefineF_contR; eauto.
+  - intros. eapply SimF_contR; eauto.
   Unshelve. all: exact None.
 Qed.
 
@@ -326,18 +321,18 @@ Lemma BisimF_index_insensitive {R1 R2 E φ sim} (POSTFIX : sim <4= BisimF φ sim
     BisimF φ sim p1' p2' t1 t2.
 Proof.
   intros. destruct REFINE.
-  split; eapply RefineF_index_insensitive; eauto; intros; apply POSTFIX; auto.
+  split; eapply SimF_index_insensitive; eauto; intros; apply POSTFIX; auto.
 Qed.
 
-Definition Refine_index_insensitive {R1 R2 E} φ :
-  ∀ p1 p2 (t1 : CTree' E R1) (t2 : CTree' E R2) (REFINE : Refine φ p1 p2 t1 t2)
+Definition Sim_index_insensitive {R1 R2 E} φ :
+  ∀ p1 p2 (t1 : CTree' E R1) (t2 : CTree' E R2) (REFINE : Sim φ p1 p2 t1 t2)
     p1' p2',
-    Refine φ p1' p2' t1 t2.
+    Sim φ p1' p2' t1 t2.
 Proof.
-  pose proof (RefineF_index_insensitive (E := E) (Refine_postfix φ)).
+  pose proof (SimF_index_insensitive (E := E) (Sim_postfix φ)).
   intros. punfold REFINE. pfold.
-  eapply RefineF_monotone.
-  { eapply H. eapply RefineF_monotone; eauto. intros. pclearbot. auto. }
+  eapply SimF_monotone.
+  { eapply H. eapply SimF_monotone; eauto. intros. pclearbot. auto. }
   eauto.
 Qed.
 
@@ -353,8 +348,8 @@ Proof.
   eauto.
 Qed.
 
-Lemma Refine_refl {R E} φ (R_REFL : ∀ v, φ v v) :
-  ∀ p1 p2 (t : CTree' E R), Refine φ p1 p2 t t.
+Lemma Sim_refl {R E} φ (R_REFL : ∀ v, φ v v) :
+  ∀ p1 p2 (t : CTree' E R), Sim φ p1 p2 t t.
 Proof.
   pcofix CIH.
   intros. pfold. destruct t.
@@ -383,19 +378,19 @@ Proof.
   Unshelve. all: exact None.
 Qed.
 
-Lemma Refine_inv_retL E R0 R1 R2
+Lemma Sim_inv_retL E R0 R1 R2
   (φ0 : R0 → R2 → Prop) (φ1 : R1 → R2 → Prop)
   (sim0 : _ → _ → _ → _ → Prop)
-  (POSTFIX : sim0 <4= RefineF φ0 sim0)
+  (POSTFIX : sim0 <4= SimF φ0 sim0)
   (sim1 : _ → _ → _ → _ → Prop) :
-  ∀ p0' p1' t0 t1 (REFINE : RefineF (E := E) φ0 sim0 p0' p1' t0 t1) t0' r0 r1
+  ∀ p0' p1' t0 t1 (REFINE : SimF (E := E) φ0 sim0 p0' p1' t0 t1) t0' r0 r1
     (IMPLφ : ∀ r2, φ0 r0 r2 → φ1 r1 r2)
     (OBS0 : t0 = Ret r0) (OBS0' : t0' = Ret r1)
     p0 p1,
-    RefineF (E := E) φ1 sim1 p0 p1 t0' t1.
+    SimF (E := E) φ1 sim1 p0 p1 t0' t1.
 Proof.
   do 5 intro.
-  apply RefineF_index_insensitive with (p1' := Some 0) (p2' := p1') in REFINE; auto.
+  apply SimF_index_insensitive with (p1' := Some 0) (p2' := p1') in REFINE; auto.
   clear p0'. remember (Some 0) as p0' in REFINE. revert Heqp0'.
   induction REFINE.
   - intros; subst. cbv in LT1. destruct p1'; lia.
@@ -408,19 +403,19 @@ Proof.
   Unshelve. exact None.
 Qed.
 
-Lemma Refine_inv_retR E R0 R1 R2
+Lemma Sim_inv_retR E R0 R1 R2
   (φ0 : R0 → R1 → Prop) (φ1 : R0 → R2 → Prop)
   (sim0 : _ → _ → _ → _ → Prop)
-  (POSTFIX : sim0 <4= RefineF φ0 sim0)
+  (POSTFIX : sim0 <4= SimF φ0 sim0)
   (sim1 : _ → _ → _ → _ → Prop) :
-  ∀ p0' p1' t0 t1 (REFINE : RefineF (E := E) φ0 sim0 p0' p1' t0 t1) t1' r1 r2
+  ∀ p0' p1' t0 t1 (REFINE : SimF (E := E) φ0 sim0 p0' p1' t0 t1) t1' r1 r2
     (IMPLφ : ∀ r0, φ0 r0 r1 → φ1 r0 r2)
     (OBS0 : t1 = Ret r1) (OBS0' : t1' = Ret r2)
     p0 p1,
-    RefineF (E := E) φ1 sim1 p0 p1 t0 t1'.
+    SimF (E := E) φ1 sim1 p0 p1 t0 t1'.
 Proof.
   do 5 intro.
-  apply RefineF_index_insensitive with (p1' := p0') (p2' := Some 0) in REFINE; auto.
+  apply SimF_index_insensitive with (p1' := p0') (p2' := Some 0) in REFINE; auto.
   clear p1'. remember (Some 0) as p1' in REFINE. revert Heqp1'.
   induction REFINE.
   - intros; subst. cbv in LT2. destruct p2'; lia.
@@ -433,16 +428,16 @@ Proof.
   Unshelve. exact None.
 Qed.
 
-Lemma Refine_inv_zeroR E R0 R1 R2 sim (sim' : _ → _ → _ → _ → Prop)
+Lemma Sim_inv_zeroR E R0 R1 R2 sim (sim' : _ → _ → _ → _ → Prop)
   (φ : R0 → R1 → Prop) (φ' : R0 → R2 → Prop)
-  (POSTFIX : sim <4= RefineF φ sim) :
-  ∀ p0 p1 t0 t1 (REFINE : RefineF (E := E) φ sim p0 p1 t0 t1)
+  (POSTFIX : sim <4= SimF φ sim) :
+  ∀ p0 p1 t0 t1 (REFINE : SimF (E := E) φ sim p0 p1 t0 t1)
     (OBS0 : t1 = Zero)
     p0' p1' t1',
-    RefineF (E := E) φ' sim' p0' p1' t0 t1'.
+    SimF (E := E) φ' sim' p0' p1' t0 t1'.
 Proof.
   do 5 intro.
-  apply RefineF_index_insensitive with (p1' := p0) (p2' := Some 0) in REFINE; auto.
+  apply SimF_index_insensitive with (p1' := p0) (p2' := Some 0) in REFINE; auto.
   remember (Some 0) as p1' in REFINE.
   revert Heqp1'. clear p1.
   induction REFINE.
@@ -455,17 +450,17 @@ Proof.
   Unshelve. all:exact None.
 Qed.
 
-Lemma Refine_inv_choiceL E R0 R1 sim (φ : R0 → R1 → Prop)
-  (POSTFIX : sim <4= RefineF φ sim) :
-  ∀ p0 p1 t0 t1 (REFINE : RefineF (E := E) φ sim p0 p1 t0 t1)
+Lemma Sim_inv_choiceL E R0 R1 sim (φ : R0 → R1 → Prop)
+  (POSTFIX : sim <4= SimF φ sim) :
+  ∀ p0 p1 t0 t1 (REFINE : SimF (E := E) φ sim p0 p1 t0 t1)
     k (OBS0 : t0 = Choice k)
     c,
-    RefineF (E := E) φ sim p0 p1 (obs_ctree (k c)) t1.
+    SimF (E := E) φ sim p0 p1 (obs_ctree (k c)) t1.
 Proof.
   do 5 intro.
-  apply RefineF_index_insensitive with (p1' := Some 0) (p2' := p1) in REFINE; auto.
+  apply SimF_index_insensitive with (p1' := Some 0) (p2' := p1) in REFINE; auto.
   intros.
-  apply RefineF_index_insensitive with (p1 := Some 0) (p2 := p1); auto.
+  apply SimF_index_insensitive with (p1 := Some 0) (p2 := p1); auto.
   clear p0. revert p1 t0 t1 REFINE k OBS0 c.
   remember (Some 0) as p0. do 4 intro. revert Heqp0.
   induction REFINE.
@@ -474,43 +469,204 @@ Proof.
   - inversion 2.
   - inversion 2.
   - inversion 2; subst; clear_sig.
-    intros. eapply RefineF_index_insensitive; eauto.
+    intros. eapply SimF_index_insensitive; eauto.
   - intros; subst.
     exploit IHREFINE; eauto. instantiate (1 := c0).
     intros.
     econstructor 6; eauto.
 Qed.
 
-(*
-  RefineF φ sim p1 p2 t1 t2 ↔
-  ∀ p1' t1', t1 => t1' → ∃ p2' t2', t2 =>* t2' ∧ sim p1' p2' t1' t2'
-  and
-  ∀ p1' t1' ℓ, t1 =ℓ=> t1' → ∃ p2' t2', t2 =>*ℓ=>* t2' ∧ sim p1' p2' t1' t2'
-  and
-  ∀ r1, t1 ⇓ r1 → ∃ t2' r2, t2 =>* t2' ∧ t2' ⇓ r2 ∧ φ r1 r2
-*)
+Lemma Sim_inv_divL E R0 R1 sim (φ : R0 → R1 → Prop)
+  (POSTFIX : sim <4= SimF φ sim) :
+  ∀ p0 p1 t0 t1 (REFINE : SimF (E := E) φ sim p0 p1 t0 t1)
+    (DIV0 : div t0),
+    div t1.
+Proof.
+  pcofix CIH.
+  do 5 intro.
+  apply SimF_index_insensitive with (p1' := p0) (p2' := Some 0) in REFINE; auto.
+  clear p1. remember (Some 0) as p1 in REFINE. revert Heqp1.
+  induction REFINE; intros; subst; try solve [punfold DIV0; inversion DIV0].
+  - cbv in LT2. destruct p2'; lia.
+  - punfold DIV0; inversion DIV0; subst; pclearbot; eauto.
+  - pfold. econstructor; eauto.
+Qed.
 
-(* RefineF φ12 sim12 p11 p12 t1 t2 *)
-(* RefineF φ23 sim23 p21 p22 t2 t3 *)
-(* does not imply RefineF (comp2 φ12 φ23) (comp4 sim12 sim23) p11 p22 t1 t3 *)
-(* this is because of the silent steps *)
+Variant State {E : Type → Type} {R : Type} :=
+| IntS (t : CTree' E R) (* internal activity *)
+| ExtS {A} (k : A → CTree E R) (* waiting for external response *)
+.
 
-Lemma RefineF_transL {R1 R2 R3 E} (φ12 : R1 → R2 → Prop) (φ23 : R2 → R3 → Prop)
-  sim12 sim23
-  (POSTFIX12 : sim12 <4= RefineF (E := E) φ12 sim12)
-  (POSTFIX23 : sim23 <4= RefineF (E := E) φ23 sim23) :
-  ∀ p11 p12 t1 t2 (REFINE1 : RefineF (E := E) φ12 sim12 p11 p12 t1 t2)
-    p21 p22 t3 (REFINE2 : RefineF (E := E) φ23 sim23 p21 p22 t2 t3),
-    RefineF (comp2 φ12 φ23) (comp4 (RefineF φ12 sim12) sim23) p11 p22 t1 t3.
+Arguments State : clear implicits.
+
+Variant Label {E : Type → Type} {R : Type} :=
+| RetL (r : R)
+| QueL {A} (e : E A)
+| AnsL {A} (a : A)
+| TauL
+.
+
+Arguments Label : clear implicits.
+
+(* we emit a τ only when the path taken may diverge *)
+Inductive Step {E : Type → Type} {R : Type}
+: State E R → Label E R → State E R → Prop :=
+| RetStep r
+: Step (IntS (Ret r)) (RetL r) (IntS Zero)
+| VisStep {A} (e : E A) k
+: Step (IntS (Vis e k)) (QueL e) (ExtS k)
+| AnsStep {A} k (a : A)
+: Step (ExtS k) (AnsL a) (IntS (obs_ctree (k a)))
+| DivStep k (DIV : div (Choice k))
+: Step (IntS (Choice k)) TauL (IntS (Choice k))
+| ChoiceStep k c ℓ s' (STEP : Step (IntS (obs_ctree (k c))) ℓ s')
+: Step (IntS (Choice k)) ℓ s'
+.
+
+Section IND.
+  Context {R : Type} {E : Type → Type}.
+  Context (P : ∀ s ℓ s', @Step E R s ℓ s' → Prop).
+  Context (PRetStep : ∀ r, P _ _ _ (RetStep r))
+          (PVisStep : ∀ {A} (e : E A) k, P _ _ _ (VisStep e k))
+          (PAnsStep : ∀ {A} k (a : A), P _ _ _ (AnsStep k a))
+          (PDivStep : ∀ k DIV, P _ _ _ (DivStep k DIV))
+          (PChoiceStep : ∀ k c ℓ s' STEP (IHSTEPk : P _ _ _ STEP), P _ _ _ (ChoiceStep k c ℓ s' STEP)).
+  Fixpoint Step_ind s ℓ s' pf : P s ℓ s' pf.
+  Proof.
+    destruct pf.
+    - apply PRetStep.
+    - apply PVisStep.
+    - apply PAnsStep.
+    - apply PDivStep.
+    - apply PChoiceStep. apply Step_ind.
+  Qed.
+End IND.
+
+Definition RelLabel {E R1 R2} (φ : R1 → R2 → Prop) (ℓ1 : Label E R1) (ℓ2 : Label E R2) :=
+  match ℓ1 with
+  | RetL r1 => match ℓ2 with RetL r2 => φ r1 r2 | _ => False end
+  | QueL e1 => match ℓ2 with QueL e2 => existT _ _ e1 = existT _ _ e2 | _ => False end
+  | AnsL a1 => match ℓ2 with AnsL a2 => existT _ _  a1 = existT _ _ a2 | _ => False end
+  | TauL => match ℓ2 with TauL => True | _ => False end
+  end.
+
+Definition SimLTSF {E R1 R2} (φ : R1 → R2 → Prop)
+  (sim : State E R1 → State E R2 → Prop) s1 s2 :=
+  ∀ ℓ1 s1' (STEP1 : Step s1 ℓ1 s1'),
+    ∃ ℓ2 s2', RelLabel φ ℓ1 ℓ2 ∧ Step s2 ℓ2 s2' ∧ sim s1' s2'
+.
+
+Variant lift_sim {E R1 R2 φ sim} : State E R1 → State E R2 → Prop :=
+| sim_Int p1 p2 t1 t2
+  (SIM : SimF φ sim p1 p2 t1 t2)
+: lift_sim (IntS t1) (IntS t2)
+| sim_Ext {A} (p1 p2 : option nat) k1 k2
+  (SIM : ∀ a : A, sim p1 p2 (obs_ctree (k1 a)) (obs_ctree (k2 a)))
+: lift_sim (ExtS k1) (ExtS k2)
+.
+
+Arguments lift_sim {_ _ _} _ _.
+
+Lemma SimF_SimLTSF {E R1 R2}
+  (φ : R1 → R2 → Prop) sim (POSTFIX : sim <4= SimF (E := E) φ sim) :
+  ∀ p1 p2 t1 t2 (SIM : SimF φ sim p1 p2 t1 t2),
+    SimLTSF φ (lift_sim φ sim) (IntS t1) (IntS t2).
+Proof.
+  intros.
+  apply SimF_index_insensitive with (p1' := Some 0) (p2' := p2) in SIM; auto.
+  clear p1. remember (Some 0) as p1. revert Heqp1.
+  induction SIM; intros; subst.
+  - cbv in LT1. destruct p1'; lia.
+  - red. inversion 1; subst.
+    exists (RetL y), (IntS Zero).
+    constructor. eauto.
+    constructor. repeat constructor.
+    econstructor. econstructor 4.
+  - red. inversion 1; subst; clear_sig.
+    exists (QueL e), (ExtS k2).
+    repeat econstructor; eauto.
+  - red. inversion 1.
+  - repeat intro. clear IHk.
+    remember (IntS (Choice k)) as s1 in STEP1.
+    assert match s1 with
+    | IntS (Choice k) => ∀ n, SimF φ sim p1' p2 (obs_ctree (k n)) t2
+    | _ => False
+    end by (subst; auto).
+    clear Heqs1 CHOICE k.
+    rename H into CHOICE.
+    revert CHOICE.
+    induction STEP1; try solve [destruct 1]; intros.
+    { punfold DIV. inversion DIV; subst. pclearbot.
+      specialize (CHOICE c) as CHOICE'.
+      eapply Sim_inv_divL in CHOICE' as DIV'; eauto.
+      punfold DIV'. inversion DIV'; subst. pclearbot. clear DIV'.
+      exists TauL, (IntS (Choice k0)).
+      split. cbv; auto.
+      split. constructor. pfold; econstructor; eauto.
+      econstructor. econstructor 5; eauto. }
+    { specialize (CHOICE c). destruct (obs_ctree (k c)).
+      { inversion STEP1; subst. clear STEP1 IHSTEP1.
+        remember (Ret v) as t1 in CHOICE.
+        apply SimF_index_insensitive with (p1' := Some 0) (p2' := p2) in CHOICE; auto.
+        clear p1'.
+        remember (Some 0) as p1. revert Heqt1 Heqp1.
+        induction CHOICE; try solve [inversion 1].
+        { intros; subst. cbv in LT1. destruct p1'; lia. }
+        { inversion 1; intros; subst.
+          exists (RetL y), (IntS Zero).
+          constructor; eauto.
+          constructor. repeat econstructor; eauto.
+          econstructor. econstructor 4; eauto. }
+        { intros; subst.
+          destruct (IHCHOICE eq_refl eq_refl) as (ℓ2 & s2' & ? & ? & ?).
+          exists ℓ2, s2'.
+          constructor; eauto.
+          constructor; eauto.
+          econstructor 5; eauto. } }
+      { inversion STEP1; subst; clear_sig. clear STEP1 IHSTEP1.
+        remember (Vis e k0) as t1 in CHOICE.
+        apply SimF_index_insensitive with (p1' := Some 0) (p2' := p2) in CHOICE; auto.
+        clear p1'.
+        remember (Some 0) as p1. revert Heqt1 Heqp1.
+        induction CHOICE; try solve [inversion 1].
+        { intros; subst. cbv in LT1. destruct p1'; lia. }
+        { inversion 1; intros; subst; clear_sig.
+          exists (QueL e), (ExtS k2).
+          repeat econstructor; eauto. }
+        { intros; subst.
+          destruct (IHCHOICE eq_refl eq_refl) as (ℓ2 & s2' & ? & ? & ?).
+          exists ℓ2, s2'.
+          constructor; eauto.
+          constructor; eauto.
+          econstructor 5; eauto. } }
+      { inversion STEP1. }
+      { apply IHSTEP1. intros. eapply Sim_inv_choiceL; eauto. } }
+  - red. intros. specialize (IHSIM eq_refl _ _ STEP1).
+    destruct IHSIM as (ℓ2 & s2' & ? & ? & ?).
+    exists ℓ2, s2'.
+    constructor; eauto.
+    constructor; eauto.
+    econstructor 5; eauto.
+  Unshelve. all: exact None.
+Qed.
+
+(* why separate φ and sim when sim is enough to express the relation between return values? *)
+Lemma SimF_transL {R1 R2 R3 E}
+  (φ12 : R1 → R2 → Prop) (φ23 : R2 → R3 → Prop) sim12 sim23
+  (POSTFIX12 : sim12 <4= SimF (E := E) φ12 sim12)
+  (POSTFIX23 : sim23 <4= SimF (E := E) φ23 sim23) :
+  ∀ p11 p12 t1 t2 (REFINE1 : SimF (E := E) φ12 sim12 p11 p12 t1 t2)
+    p21 p22 t3 (REFINE2 : SimF (E := E) φ23 sim23 p21 p22 t2 t3),
+    SimF (comp2 φ12 φ23) (comp4 (SimF φ12 sim12) sim23) p11 p22 t1 t3.
 Proof.
   do 5 intro. induction REFINE1.
   - do 4 intro. apply POSTFIX12 in SIM. revert t1 SIM. induction REFINE2.
     { intros. econstructor 1; cbv [comp4]; eauto. }
     { intros.
-      eapply Refine_inv_retR; first [eassumption | reflexivity | idtac].
+      eapply Sim_inv_retR; first [eassumption | reflexivity | idtac].
       cbv [comp2]; eauto. }
     { intros.
-      apply RefineF_index_insensitive with (p1' := Some 0) (p2' := Some 0) in SIM; auto.
+      apply SimF_index_insensitive with (p1' := Some 0) (p2' := Some 0) in SIM; auto.
       remember (Some 0) as o' in SIM. revert Heqo'.
       remember (Vis e k1) as t2 in SIM. revert Heqt2.
       induction SIM.
@@ -522,9 +678,9 @@ Proof.
       { intros. subst. econstructor 4; eauto. }
       { intros; subst. econstructor 5; eauto. }
       { inversion 1. } }
-    { intros. eapply Refine_inv_zeroR; eauto. }
+    { intros. eapply Sim_inv_zeroR; eauto. }
     { intros.
-      apply RefineF_index_insensitive with (p1' := Some 0) (p2' := Some 0) in SIM; auto.
+      apply SimF_index_insensitive with (p1' := Some 0) (p2' := Some 0) in SIM; auto.
       remember (Some 0) as o' in SIM. revert Heqo'.
       remember (Choice k) as t2' in SIM. revert Heqt2'.
       induction SIM.
@@ -534,13 +690,13 @@ Proof.
       { intros. subst. econstructor 4; eauto. }
       { intros. subst. econstructor 5; eauto. }
       { inversion 1; intros; subst. clear_sig. apply (IHk c).
-        eapply RefineF_index_insensitive; eauto. } }
+        eapply SimF_index_insensitive; eauto. } }
     { intros. econstructor 6; eauto. }
   - intros; subst.
-    eapply Refine_inv_retL; first [eassumption | reflexivity | idtac].
+    eapply Sim_inv_retL; first [eassumption | reflexivity | idtac].
     cbv [comp2]. eauto.
   - intros.
-    apply RefineF_index_insensitive with (p1' := Some 0) (p2' := p22) in REFINE2; auto.
+    apply SimF_index_insensitive with (p1' := Some 0) (p2' := p22) in REFINE2; auto.
     remember (Some 0) as o' in REFINE2. revert Heqo'.
     remember (Vis e k2) as t2 in REFINE2. revert Heqt2.
     induction REFINE2.
@@ -556,26 +712,25 @@ Proof.
     { intros. econstructor 6; eauto. }
   - intros. econstructor 4; eauto.
   - intros. econstructor 5; eauto.
-  - intros. eapply IHREFINE1. eapply Refine_inv_choiceL in REFINE2; eauto.
+  - intros. eapply IHREFINE1. eapply Sim_inv_choiceL in REFINE2; eauto.
 Qed.
 
-Lemma RefineF_transR {R1 R2 R3 E} (φ12 : R1 → R2 → Prop) (φ23 : R2 → R3 → Prop)
-  sim12 sim23
-  (POSTFIX12 : sim12 <4= RefineF (E := E) φ12 sim12)
-  (POSTFIX23 : sim23 <4= RefineF (E := E) φ23 sim23) :
-  ∀ p11 p12 t1 t2 (REFINE1 : RefineF (E := E) φ12 sim12 p11 p12 t1 t2)
-    p21 p22 t3 (REFINE2 : RefineF (E := E) φ23 sim23 p21 p22 t2 t3),
-    RefineF (comp2 φ12 φ23) (comp4 sim12 (RefineF φ23 sim23)) p11 p22 t1 t3.
+Lemma SimF_transR {R1 R2 R3 E}
+  (φ12 : R1 → R2 → Prop) (φ23 : R2 → R3 → Prop) sim12 sim23
+  (POSTFIX12 : sim12 <4= SimF (E := E) φ12 sim12)
+  (POSTFIX23 : sim23 <4= SimF (E := E) φ23 sim23) :
+  ∀ p11 p12 t1 t2 (REFINE1 : SimF (E := E) φ12 sim12 p11 p12 t1 t2)
+    p21 p22 t3 (REFINE2 : SimF (E := E) φ23 sim23 p21 p22 t2 t3),
+    SimF (comp2 φ12 φ23) (comp4 sim12 (SimF φ23 sim23)) p11 p22 t1 t3.
 Proof.
   do 9 intro. revert p11 p12 t1 REFINE1. induction REFINE2.
   - do 4 intro. apply POSTFIX23 in SIM. revert t2 SIM. induction REFINE1.
     { intros. econstructor 1; cbv [comp4]; eauto. }
-    { intros. eapply Refine_inv_retL; eauto.
+    { intros. eapply Sim_inv_retL; eauto.
       cbv [comp2]; eauto. }
     { intros. clear LT1 LT2 p1 p3.
-      apply RefineF_index_insensitive with (p1' := Some 0) (p2' := Some 1) in SIM; auto.
+      apply SimF_index_insensitive with (p1' := Some 0) (p2' := p2') in SIM; auto.
       remember (Some 0) as o' in SIM. revert Heqo'.
-      remember (Some 1) as o'' in SIM. clear Heqo''.
       remember (Vis e k2) as t1 in SIM. revert Heqt1.
       induction SIM.
       { intros; subst. cbv in LT1. destruct p1'1; lia. }
@@ -589,12 +744,11 @@ Proof.
       { intros. subst. econstructor 6; eauto. } }
     { intros. econstructor 4; eauto. }
     { intros. econstructor 5; eauto. }
-    { intros. clear p3. rename p2'0 into p3.
-      apply IHREFINE1. eapply Refine_inv_choiceL; eauto. }
-  - intros; subst. eapply Refine_inv_retR; eauto.
+    { intros. eauto using Sim_inv_choiceL. }
+  - intros; subst. eapply Sim_inv_retR; eauto.
     cbv [comp2]. eauto.
   - intros.
-    apply RefineF_index_insensitive with (p1' := p11) (p2' := Some 0) in REFINE1; auto.
+    apply SimF_index_insensitive with (p1' := p11) (p2' := Some 0) in REFINE1; auto.
     remember (Some 0) as o' in REFINE1. revert Heqo'.
     remember (Vis e k1) as t2 in REFINE1. revert Heqt2.
     induction REFINE1.
@@ -608,9 +762,9 @@ Proof.
     { intros. econstructor 4; eauto. }
     { intros. econstructor 5; eauto. }
     { inversion 1. }
-  - intros. eapply Refine_inv_zeroR; eauto.
+  - intros. eapply Sim_inv_zeroR; eauto.
   - intros.
-    apply RefineF_index_insensitive with (p1' := p11) (p2' := Some 0) in REFINE1; auto.
+    apply SimF_index_insensitive with (p1' := p11) (p2' := Some 0) in REFINE1; auto.
     remember (Some 0) as o' in REFINE1. revert Heqo'.
     remember (Choice k) as t2' in REFINE1. revert Heqt2'.
     induction REFINE1.
@@ -624,22 +778,21 @@ Proof.
 Qed.
 
 Lemma BisimF_trans_not_choice {R1 R2 R3 E}
-  (φ12 : R1 → R2 → Prop) (φ23 : R2 → R3 → Prop)
-  sim12 sim23
-  (POSTFIX12 : sim12 <4= RefineF (E := E) φ12 sim12)
-  (POSTFIX23 : sim23 <4= RefineF (E := E) φ23 sim23) :
-  ∀ p11 p12 t1 t2 (REFINE1 : RefineF (E := E) φ12 sim12 p11 p12 t1 t2)
-    p21 p22 t3 (REFINE2 : RefineF (E := E) φ23 sim23 p21 p22 t2 t3)
+  (φ12 : R1 → R2 → Prop) (φ23 : R2 → R3 → Prop) sim12 sim23
+  (POSTFIX12 : sim12 <4= SimF (E := E) φ12 sim12)
+  (POSTFIX23 : sim23 <4= SimF (E := E) φ23 sim23) :
+  ∀ p11 p12 t1 t2 (REFINE1 : SimF (E := E) φ12 sim12 p11 p12 t1 t2)
+    p21 p22 t3 (REFINE2 : SimF (E := E) φ23 sim23 p21 p22 t2 t3)
     (NCHOICE : match t2 with Choice _ => False | _ => True end),
-    RefineF (comp2 φ12 φ23) (comp4 sim12 sim23) p11 p22 t1 t3.
+    SimF (comp2 φ12 φ23) (comp4 sim12 sim23) p11 p22 t1 t3.
 Proof.
   do 9 intro. revert p11 p12 t1 REFINE1. induction REFINE2.
   - do 4 intro. revert t2 SIM. induction REFINE1.
     { intros. econstructor 1; cbv [comp4]; eauto. }
-    { intros. eapply Refine_inv_retL; eauto.
+    { intros. eapply Sim_inv_retL; eauto.
       cbv [comp2]; eauto. }
     { intros. clear LT1 LT2 p1 p3. apply POSTFIX23 in SIM.
-      apply RefineF_index_insensitive with (p1' := Some 0) (p2' := Some 1) in SIM; auto.
+      apply SimF_index_insensitive with (p1' := Some 0) (p2' := Some 1) in SIM; auto.
       remember (Some 0) as o' in SIM. revert Heqo'.
       remember (Some 1) as o'' in SIM. clear Heqo''.
       remember (Vis e k2) as t1 in SIM. revert Heqt1.
@@ -655,10 +808,10 @@ Proof.
     { intros. econstructor 4; eauto. }
     { intros. econstructor 5; eauto. }
     { destruct 2. }
-  - intros; subst. eapply Refine_inv_retR; eauto.
+  - intros; subst. eapply Sim_inv_retR; eauto.
     cbv [comp2]. eauto.
   - intros.
-    apply RefineF_index_insensitive with (p1' := p11) (p2' := Some 0) in REFINE1; auto.
+    apply SimF_index_insensitive with (p1' := p11) (p2' := Some 0) in REFINE1; auto.
     remember (Some 0) as o' in REFINE1. revert Heqo'.
     remember (Vis e k1) as t2 in REFINE1. revert Heqt2.
     induction REFINE1.
@@ -671,27 +824,26 @@ Proof.
     { intros. econstructor 4; eauto. }
     { intros. econstructor 5; eauto. }
     { inversion 1. }
-  - intros. eapply Refine_inv_zeroR; eauto.
+  - intros. eapply Sim_inv_zeroR; eauto.
   - destruct 2.
   - intros. econstructor 6; eauto.
 Qed.
 
 Lemma BisimF_trans {R1 R2 R3 E}
-  (φ12 : R1 → R2 → Prop) (φ23 : R2 → R3 → Prop)
-  sim12 sim23
-  (POSTFIX12 : sim12 <4= RefineF (E := E) φ12 sim12)
-  (POSTFIX23 : sim23 <4= RefineF (E := E) φ23 sim23) :
-  ∀ p11 p12 t1 t2 (REFINE1 : RefineF (E := E) φ12 sim12 p11 p12 t1 t2)
-    p21 p22 t3 (REFINE2 : RefineF (E := E) φ23 sim23 p21 p22 t2 t3),
-    RefineF (comp2 φ12 φ23) (comp4 sim12 sim23) p11 p22 t1 t3.
+  (φ12 : R1 → R2 → Prop) (φ23 : R2 → R3 → Prop) sim12 sim23
+  (POSTFIX12 : sim12 <4= SimF (E := E) φ12 sim12)
+  (POSTFIX23 : sim23 <4= SimF (E := E) φ23 sim23) :
+  ∀ p11 p12 t1 t2 (REFINE1 : SimF (E := E) φ12 sim12 p11 p12 t1 t2)
+    p21 p22 t3 (REFINE2 : SimF (E := E) φ23 sim23 p21 p22 t2 t3),
+    SimF (comp2 φ12 φ23) (comp4 sim12 sim23) p11 p22 t1 t3.
 Proof.
   do 9 intro. revert p11 p12 t1 REFINE1. induction REFINE2.
   - do 4 intro. revert t2 SIM. induction REFINE1.
     { intros. econstructor 1; cbv [comp4]; eauto. }
-    { intros. eapply Refine_inv_retL; eauto.
+    { intros. eapply Sim_inv_retL; eauto.
       cbv [comp2]; eauto. }
     { intros. clear LT1 LT2 p1 p3. apply POSTFIX23 in SIM.
-      apply RefineF_index_insensitive with (p1' := Some 0) (p2' := p2') in SIM; auto.
+      apply SimF_index_insensitive with (p1' := Some 0) (p2' := p2') in SIM; auto.
       remember (Some 0) as o' in SIM. revert Heqo'.
       remember (Vis e k2) as t1 in SIM. revert Heqt1.
       induction SIM.
@@ -706,10 +858,10 @@ Proof.
     { intros. econstructor 4; eauto. }
     { intros. econstructor 5; eauto. }
     { admit. }
-  - intros; subst. eapply Refine_inv_retR; eauto. 
+  - intros; subst. eapply Sim_inv_retR; eauto. 
     cbv [comp2]. eauto.
   - intros.
-    apply RefineF_index_insensitive with (p1' := p11) (p2' := Some 0) in REFINE1; auto.
+    apply SimF_index_insensitive with (p1' := p11) (p2' := Some 0) in REFINE1; auto.
     remember (Some 0) as o' in REFINE1. revert Heqo'.
     remember (Vis e k1) as t2 in REFINE1. revert Heqt2.
     induction REFINE1.
@@ -722,9 +874,9 @@ Proof.
     { intros. econstructor 4; eauto. }
     { intros. econstructor 5; eauto. }
     { inversion 1. }
-  - intros. eapply Refine_inv_zeroR; eauto.
+  - intros. eapply Sim_inv_zeroR; eauto.
   - intros.
-    apply RefineF_index_insensitive with (p1' := p11) (p2' := Some 0) in REFINE1; auto.
+    apply SimF_index_insensitive with (p1' := p11) (p2' := Some 0) in REFINE1; auto.
     remember (Some 0) as o' in REFINE1. revert Heqo'.
     remember (Choice k) as t2' in REFINE1. revert Heqt2'.
     induction REFINE1.
@@ -740,12 +892,12 @@ Abort.
 Lemma BisimF_trans_choice {R1 R2 R3 E}
   (φ12 : R1 → R2 → Prop) (φ23 : R2 → R3 → Prop)
   sim12 sim23
-  (POSTFIX12 : sim12 <4= RefineF (E := E) φ12 sim12)
-  (POSTFIX23 : sim23 <4= RefineF (E := E) φ23 sim23) :
-  ∀ p11 p12 t1 t2 (REFINE1 : RefineF (E := E) φ12 sim12 p11 p12 t1 t2)
-    p21 p22 t3 (REFINE2 : RefineF (E := E) φ23 sim23 p21 p22 t2 t3)
+  (POSTFIX12 : sim12 <4= SimF (E := E) φ12 sim12)
+  (POSTFIX23 : sim23 <4= SimF (E := E) φ23 sim23) :
+  ∀ p11 p12 t1 t2 (REFINE1 : SimF (E := E) φ12 sim12 p11 p12 t1 t2)
+    p21 p22 t3 (REFINE2 : SimF (E := E) φ23 sim23 p21 p22 t2 t3)
     k (CHOICE : t2 = Choice k),
-    RefineF (comp2 φ12 φ23) (comp4 sim12 sim23) p11 p22 t1 t3.
+    SimF (comp2 φ12 φ23) (comp4 sim12 sim23) p11 p22 t1 t3.
 Proof.
   do 9 intro. revert p11 p12 t1 REFINE1. induction REFINE2.
   - intros. revert k CHOICE t2 SIM. induction REFINE1.
@@ -754,9 +906,9 @@ Proof.
     { inversion 1. }
     { intros. econstructor 4; eauto. }
     { intros; subst. econstructor 5; eauto. }
-    { inversion 1; subst; clear_sig. intros. apply POSTFIX23 in SIM.
-      eapply Refine_inv_choiceL with (c := c) in SIM; auto.
-      apply RefineF_index_insensitive with (p1' := p1') (p2' := p2) in SIM; auto.
+    { inversion 1; subst. clear CHOICE. intros. apply POSTFIX23 in SIM as REFINE2.
+      eapply Sim_inv_choiceL with (c := c) in REFINE2; auto.
+      apply SimF_index_insensitive with (p1' := p1') (p2' := p2) in REFINE2; auto.
       destruct (obs_ctree (k0 c)) eqn:OBS.
       1,2,3: eapply BisimF_trans_not_choice; eauto; simpl; auto.
       specialize (IHREFINE1 _ eq_refl). admit. }
@@ -764,7 +916,7 @@ Proof.
   - inversion 2.
   - inversion 2.
   - inversion 2; subst.
-    apply RefineF_index_insensitive with (p1' := p11) (p2' := Some 0) in REFINE1; auto.
+    apply SimF_index_insensitive with (p1' := p11) (p2' := Some 0) in REFINE1; auto.
     remember (Some 0) as o' in REFINE1. revert Heqo'.
     remember (Choice k0) as t2' in REFINE1. revert Heqt2'.
     induction REFINE1.
@@ -780,47 +932,56 @@ Proof.
   - intros; subst. econstructor 6; eauto.
 Abort.
 
-CoFixpoint infND {E R} : CTree E R :=
-  {| obs_ctree := Choice (fun _ => infND) |}
-.
-
-Variant isInfNDF {E R sim} : CTree' E R → Prop :=
-| isInfND_intro k c
-  (SIM : sim (obs_ctree (k c)) : Prop)
-: isInfNDF (Choice k)
-.
-
-Arguments isInfNDF {_ _} _ _.
-
-Lemma isInfNDF_monotone {E R} : monotone1 (@isInfNDF E R).
-Proof. repeat intro. destruct IN. econstructor; eauto. Qed.
-
-Hint Resolve isInfNDF_monotone : paco.
-
-Definition isInfND {E R} := paco1 (@isInfNDF E R) bot1.
-
-Lemma infND_refineL {E R1 R2 R} :
-  ∀ p1 p2 (t : CTree' E R2) (REFINEL : Refine R p1 p2 (obs_ctree (infND (R := R1))) t),
-    isInfND t.
+Lemma BisimF_trans_choice {R1 R2 R3 E}
+  (φ12 : R1 → R2 → Prop) (φ23 : R2 → R3 → Prop)
+  sim12 sim23
+  (POSTFIX12 : sim12 <4= SimF (E := E) φ12 sim12)
+  (POSTFIX23 : sim23 <4= SimF (E := E) φ23 sim23) :
+  ∀ p11 p12 t1 t2 (REFINE1 : SimF (E := E) φ12 sim12 p11 p12 t1 t2)
+    p21 p22 t3 (REFINE2 : SimF (E := E) φ23 sim23 p21 p22 t2 t3)
+    k (CHOICE : t2 = Choice k),
+    SimF (comp2 φ12 φ23) (comp4 sim12 sim23) p11 p22 t1 t3.
 Proof.
-  pcofix CIH. do 2 intro. revert p1.
-  induction p2 using (well_founded_induction olt_wf).
-  rename H into IHp2.
-  do 2 intro.
-  remember infND as t' eqn:RR.
-  rewrite RR in *|-.
-  intros. punfold REFINEL. cbv [rel4] in *.
-  remember (obs_ctree t') as t1 in REFINEL. revert Heqt1.
-  revert p1 p2 t t' REFINEL IHp2 RR. induction 1; intros; subst; simpl in *.
-  - pclearbot. eauto.
-  - inversion Heqt1.
-  - inversion Heqt1.
-  - inversion Heqt1.
-  - inversion Heqt1; subst. clear_sig.
-    simpl in *.
-    specialize (IHk 0).
-    eauto.
-  - pfold. econstructor; eauto. right. eapply CIH.
-    pfold. apply REFINEL.
-Qed.
+  do 5 intro. induction REFINE1.
+  - intros. revert k CHOICE t1 SIM. induction REFINE2.
+    { intros. econstructor 1; cbv [comp4]; eauto. }
+    { inversion 1. }
+    { inversion 1. }
+    { inversion 1. }
+    { inversion 1; subst. intros. apply POSTFIX12 in SIM.
+      apply SimF_index_insensitive with (p1' := p2) (p2' := Some 0) in SIM; auto.
+      clear LT2.
+      remember (Some 0) as p' in SIM. revert Heqp'.
+      remember (Choice k0) as t2' in SIM. revert Heqt2'.
+      induction SIM.
+      { intros; subst. cbv in LT2. destruct p2'0; lia. }
+      { inversion 1. }
+      { inversion 1. }
+      { intros; econstructor 4; eauto. }
+      { intros; subst. econstructor 5; eauto. }
+      { inversion 1; intros; subst. specialize (CHOICE c). specialize (IHk c).
+        apply SimF_index_insensitive with (p1' := p1) (p2' := p2') in SIM; auto.
+        destruct (obs_ctree (k0 c)).
+        1,2,3: eapply BisimF_trans_not_choice; eauto; simpl; auto.
+        specialize (IHk _ eq_refl). admit. } }
+    { intros; subst. econstructor 6; eauto. }
+  - inversion 2.
+  - inversion 2.
+  - inversion 2. econstructor 4; eauto.
+  - intros. econstructor 5; eauto.
+  - inversion 2; subst.
+    apply SimF_index_insensitive with (p1' := Some 0) (p2' := p22) in REFINE2; auto.
+    remember (Some 0) as p' in REFINE2.
+    remember (Choice k0) as t1' in REFINE2.
+    revert Heqt1' Heqp'.
+    induction REFINE2.
+    { intros; subst. cbv in LT1. destruct p1'; lia. }
+    { inversion 1. }
+    { inversion 1. }
+    { inversion 1. }
+    { inversion 1; subst. intros; subst. specialize (CHOICE0 c).
+      destruct (obs_ctree (k0 c)); eauto.
+      all: eapply BisimF_trans_not_choice; eauto; simpl; auto. }
+    { intros; econstructor 6; eauto. }
+Abort.
 
