ChoiceTrees/CTree2.v
@@ -19,6 +19,7 @@ Inductive CTreeF {E : Type → Type} {R : Type} {CTree : Type} :=
 | Vis {A} (e : E A) (k : A → CTree)
 | Zero
 | Choice (k : nat → CTreeF)
+| Tau (t : CTree)
 .
 
 Arguments CTreeF : clear implicits.
@@ -26,17 +27,12 @@ Arguments CTreeF : clear implicits.
 Section IND.
   Context {E : Type → Type} {R : Type} {CTree : Type}.
   Context (P : CTreeF E R CTree → Prop).
-  Context (PRet : ∀ v, P (Ret v))
-          (PVis : ∀ {A} (e : E A) k, P (Vis e k))
-          (PZero : P Zero)
+  Context (PNChoice : ∀ t (NCHOICE : match t with Choice _ => False | _ => True end), P t)
           (PChoice : ∀ k (IHk : ∀ c, P (k c)), P (Choice k)).
   Fixpoint CTreeF_ind t : P t.
   Proof.
-    destruct t.
-    - apply PRet.
-    - apply PVis.
-    - apply PZero.
-    - apply PChoice. intros. apply CTreeF_ind.
+    destruct t; try solve [apply PNChoice; auto].
+    apply PChoice. intros. apply CTreeF_ind.
   Qed.
 End IND.
 
@@ -45,6 +41,16 @@ CoInductive CTree {E : Type → Type} {R : Type} : Type :=
 .
 
 Arguments CTree : clear implicits.
+
+Definition bind {E R} (k : R → CTree E R) :=
+  cofix bind_ (t : CTree E R) :=
+    match obs_ctree t with
+    | Ret v => k v
+    | Vis e k => {| obs_ctree := Vis e (fun a => bind_ (k a)) |}
+    | Zero => {| obs_ctree := Zero |}
+    | Choice k => {| obs_ctree := Choice (fun c => Tau (bind_ {| obs_ctree := k c |})) |}
+    | Tau t => {| obs_ctree := Tau (bind_ t) |}
+    end.
 
 Definition CTree' E R := CTreeF E R (CTree E R).
 
@@ -117,63 +123,67 @@ Qed.
 Lemma ole_top x : ole x None.
 Proof. destruct x; cbv; eauto. Qed.
 
-(* from FreeSim (Stuttering for Free) *)
-(* infinite silent steps should be equivalent only to infinite silent steps *)
-Inductive RefineF {R1 R2 E r sim}
-  : option nat → option nat → CTree' E R1 → CTree' E R2 → Prop :=
-| refine_prog p1 p2 t1 t2 p1' p2'
-  (* only rule that strictly decrements the progress indices*)
-  (LT1 : p1' ≺ p1) (LT2 : p2' ≺ p2)
-  (SIM : sim p1' p2' t1 t2)
-: RefineF p1 p2 t1 t2
-| refine_ret p1 p2 x y
-  (RET : r x y : Prop)
-: RefineF p1 p2 (Ret x) (Ret y)
-| refine_vis p1 p2 p1' p2' {A} (e : E A) k1 k2
-  (CONT : ∀ a, sim p1' p2' (obs_ctree (k1 a)) (obs_ctree (k2 a)))
-: RefineF p1 p2 (Vis e k1) (Vis e k2)
-| refine_zero p1 p2 t2
-: RefineF p1 p2 Zero t2
-| refine_choiceL p1 p2 p1' t2 k
-  (CHOICE : ∀ c, RefineF p1' p2 (k c) t2)
-: RefineF p1 p2 (Choice k) t2
-| refine_choiceR p1 p2 p2' t1 k
-  c (CHOICE : RefineF p1 p2' t1 (k c))
-: RefineF p1 p2 t1 (Choice k)
+Inductive RefineF {R1 R2 E r sim} : CTree' E R1 → CTree' E R2 → Prop :=
+| refine_ret x y (RET : r x y : Prop)
+: RefineF (Ret x) (Ret y)
+| refine_vis {A} (e : E A) k1 k2
+  (CONT : ∀ a, sim (obs_ctree (k1 a)) (obs_ctree (k2 a)))
+: RefineF (Vis e k1) (Vis e k2)
+| refine_zero t2
+: RefineF Zero t2
+| refine_choiceL k t2
+  (CHOICE : ∀ c, RefineF (k c) t2)
+: RefineF (Choice k) t2
+| refine_choiceR t1 k
+  c (CHOICE : RefineF t1 (k c))
+: RefineF t1 (Choice k)
+| refine_tauL t1 t2
+  (TAU : RefineF (obs_ctree t1) t2)
+: RefineF (Tau t1) t2
+| refine_tauR t1 t2
+  (TAU : RefineF t1 (obs_ctree t2))
+: RefineF t1 (Tau t2)
+| refine_tauB t1 t2
+  (TAU : sim (obs_ctree t1) (obs_ctree t2))
+: RefineF (Tau t1) (Tau t2)
 .
 
 Arguments RefineF {_ _ _} _ _.
 
 Section IND.
-  Context {R1 R2 E} (r : R1 → R2 → Prop) (sim : option nat → option nat → CTree' E R1 → CTree' E R2 → Prop).
-  Context (P : ∀ p1 p2 t1 t2, RefineF r sim p1 p2 t1 t2 → Prop).
-  Context (Pprog : ∀ p1 p2 t1 t2 p1' p2' LT1 LT2 SIM, P _ _ _ _ (refine_prog p1 p2 t1 t2 p1' p2' LT1 LT2 SIM))
-          (Pret : ∀ p1 p2 x y RET, P _ _ _ _ (refine_ret p1 p2 x y RET))
-          (Pvis : ∀ p1 p2 p1' p2' A (e : E A) k1 k2 CONT, P _ _ _ _ (refine_vis p1 p2 p1' p2' e k1 k2 CONT))
-          (Pzero : ∀ p1 p2 t2, P _ _ _ _ (refine_zero p1 p2 t2))
-          (PL : ∀ p1 p2 p1' t2 k CHOICE (IHk : ∀ c, P _ _ _ _ (CHOICE c)), P _ _ _ _ (refine_choiceL p1 p2 p1' t2 k CHOICE))
-          (PR : ∀ p1 p2 p2' t1 k c CHOICE (IHk : P _ _ _ _ CHOICE), P _ _ _ _ (refine_choiceR p1 p2 p2' t1 k c CHOICE)).
-  Fixpoint RefineF_ind p1 p2 t1 t2 pf : P p1 p2 t1 t2 pf.
+  Context {R1 R2 E} (r : R1 → R2 → Prop) (sim : CTree' E R1 → CTree' E R2 → Prop).
+  Context (P : ∀ t1 t2, RefineF r sim t1 t2 → Prop).
+  Context (Pret : ∀ x y RET, P _ _ (refine_ret x y RET))
+          (Pvis : ∀ A (e : E A) k1 k2 CONT, P _ _ (refine_vis e k1 k2 CONT))
+          (Pzero : ∀ t2, P _ _ (refine_zero t2))
+          (PL : ∀ k t2 CHOICE (IHk : ∀ c, P _ _ (CHOICE c)), P _ _ (refine_choiceL k t2 CHOICE))
+          (PR : ∀ t1 k c CHOICE (IHk : P _ _ CHOICE), P _ _ (refine_choiceR t1 k c CHOICE))
+          (PL' : ∀ t1 t2 TAU (IHt : P _ _ TAU), P _ _ (refine_tauL t1 t2 TAU))
+          (PR' : ∀ t1 t2 TAU (IHt : P _ _ TAU), P _ _ (refine_tauR t1 t2 TAU))
+          (PB : ∀ t1 t2 TAU, P _ _ (refine_tauB t1 t2 TAU)).
+  Fixpoint RefineF_ind t1 t2 pf : P t1 t2 pf.
   Proof.
     destruct pf.
-    - apply Pprog.
     - apply Pret.
     - apply Pvis.
     - apply Pzero.
     - apply PL. intros. apply RefineF_ind.
     - apply PR. intros. apply RefineF_ind.
+    - apply PL'. intros. apply RefineF_ind.
+    - apply PR'. intros. apply RefineF_ind.
+    - apply PB.
   Qed.
 End IND.
 
-Definition BisimF {R1 R2 E} (φ : R1 → R2 → Prop) sim p1 p2 t1 t2 :=
-  RefineF (E := E) φ sim p1 p2 t1 t2 ∧
+Definition BisimF {R1 R2 E} (φ : R1 → R2 → Prop) sim t1 t2 :=
+  RefineF (E := E) φ sim t1 t2 ∧
   RefineF
     (fun r1 r2 => φ r2 r1)
-    (fun p1 p2 t1 t2 => sim p2 p1 t2 t1)
-    p2 p1 t2 t1
+    (fun t1 t2 => sim t2 t1)
+    t2 t1
 .
 
-Lemma RefineF_monotone R1 R2 E r : monotone4 (@RefineF R1 R2 E r).
+Lemma RefineF_monotone R1 R2 E r : monotone2 (@RefineF R1 R2 E r).
 Proof.
   repeat intro. revert r' LE. induction IN; intros.
   - econstructor 1; eauto.
@@ -182,11 +192,13 @@ Proof.
   - econstructor 4; eauto.
   - econstructor 5; eauto.
   - econstructor 6; eauto.
+  - econstructor 7; eauto.
+  - econstructor 8; eauto.
 Qed.
 
 Hint Resolve RefineF_monotone : paco.
 
-Lemma BisimF_monotone R1 R2 E φ : monotone4 (@BisimF R1 R2 E φ).
+Lemma BisimF_monotone R1 R2 E φ : monotone2 (@BisimF R1 R2 E φ).
 Proof.
   repeat intro.
   destruct IN as (IN & IN').
@@ -195,12 +207,12 @@ Qed.
 
 Hint Resolve BisimF_monotone : paco.
 
-Definition Refine {R1 R2 E} r := paco4 (@RefineF R1 R2 E r) bot4.
+Definition Refine {R1 R2 E} r := paco2 (@RefineF R1 R2 E r) bot2.
 
-Definition Bisim {R1 R2 E} r := paco4 (@BisimF R1 R2 E r) bot4.
+Definition Bisim {R1 R2 E} r := paco2 (@BisimF R1 R2 E r) bot2.
 
 Lemma Refine_postfix {R1 R2 E} (φ : R1 → R2 → Prop) :
-  Refine (E := E) φ <4= RefineF φ (Refine φ).
+  Refine (E := E) φ <2= RefineF φ (Refine φ).
 Proof.
   repeat intro. punfold PR.
   eapply RefineF_monotone; eauto.
@@ -208,7 +220,7 @@ Proof.
 Qed.
 
 Lemma Bisim_postfix {R1 R2 E} (φ : R1 → R2 → Prop) :
-  Bisim (E := E) φ <4= RefineF φ (Bisim φ).
+  Bisim (E := E) φ <2= RefineF φ (Bisim φ).
 Proof.
   repeat intro.
   punfold PR. destruct PR.
@@ -217,8 +229,8 @@ Proof.
 Qed.
 
 Lemma Bisim_postfix_flipped {R1 R2 E} (φ : R1 → R2 → Prop) :
-  (fun p1 p2 t1 t2 => Bisim (E := E) φ p2 p1 t2 t1) <4=
-  RefineF (fun r1 r2 => φ r2 r1) (fun p1 p2 t1 t2 => Bisim φ p2 p1 t2 t1).
+  (fun t1 t2 => Bisim (E := E) φ t2 t1) <2=
+  RefineF (fun r1 r2 => φ r2 r1) (fun t1 t2 => Bisim φ t2 t1).
 Proof.
   repeat intro.
   punfold PR. destruct PR.
@@ -227,421 +239,218 @@ Proof.
 Qed.
 
 Lemma BisimF_postfix {R1 R2 E} (φ : R1 → R2 → Prop) :
-  Bisim (E := E) φ <4= BisimF φ (Bisim φ).
+  Bisim (E := E) φ <2= BisimF φ (Bisim φ).
 Proof.
   repeat intro; split.
   - apply Bisim_postfix; eauto.
   - apply Bisim_postfix_flipped; eauto.
 Qed.
 
-Definition comp2 {R1 R2 R3 : Type}
+Definition comp {R1 R2 R3 : Type}
   (r12 : R1 → R2 → Prop) (r23 : R2 → R3 → Prop) v1 v3 :=
   ∃ v2, r12 v1 v2 ∧ r23 v2 v3
 .
 
-Definition comp4 {E R1 R2 R3}
-  (sim12 : option nat → option nat → CTree' E R1 → CTree' E R2 → Prop)
-  (sim23 : option nat → option nat → CTree' E R2 → CTree' E R3 → Prop)
-  p11 p22 t1 t3 :=
-  ∃ p12 p21 t2, sim12 p11 p12 t1 t2 ∧ sim23 p21 p22 t2 t3
-.
-
-Lemma RefineF_index_mono {R1 R2 E} φ (sim : _ → _ → _ → _ → Prop) :
-  ∀ p1 p2 (t1 : CTree' E R1) (t2 : CTree' E R2) (REFINE : RefineF φ sim p1 p2 t1 t2)
-    p1' p2' (LE1 : p1 ≼ p1') (LE2 : p2 ≼ p2'),
-    RefineF φ sim p1' p2' t1 t2.
-Proof.
-  do 4 intro. induction 1.
-  - intros p1'' p2'' ? ?.
-    econstructor 1; eauto.
-    destruct LE1; subst; eauto. eapply olt_transitive; eauto.
-    destruct LE2; subst; eauto. eapply olt_transitive; eauto.
-  - intros. econstructor 2; eauto.
-  - intros. econstructor 3; eauto.
-  - intros. econstructor 4; eauto. 
-  - intros. econstructor 5; eauto.
-    intros. eapply IHk; eauto. right; auto.
-  - intros. econstructor 6; eauto.
-    intros. eapply IHREFINE; eauto. right; auto.
-Qed.
-
-Lemma RefineF_contR {R1 R2 E φ sim} (POSTFIX : sim <4= RefineF φ sim) :
-  ∀ p1 p2 (t1 : CTree' E R1) (t2' : CTree' E R2)
-    (* if t1 refines t2', *)
-    (REFINE : RefineF φ sim p1 p2 t1 t2')
-    (* for any t2 that may continue as t2', *)
-    t2 k2 (OBS : t2 = Choice k2) c2 (BR : t2' = k2 c2)
-    (* t1 must refine t2 *)
-    p1' p2', RefineF φ sim p1' p2' t1 t2.
-Proof.
-  induction p1 using (well_founded_induction olt_wf).
-  rename H into IHp1.
-  do 4 intro. revert IHp1.
-  induction REFINE; intros; subst.
-  - eauto.
-  - econstructor 6; eauto. rewrite <- BR.
-    econstructor 2; eauto.
-  - econstructor 6; eauto. rewrite <- BR.
-    econstructor 3; eauto.
-  - econstructor 4; eauto.
-  - econstructor 6; eauto. instantiate (1 := c2).
-    econstructor 5; eauto.
-  - econstructor 6; eauto.
-  Unshelve. all: exact None.
-Qed.
-
-Lemma RefineF_index_insensitive {R1 R2 E φ sim} (POSTFIX : sim <4= RefineF φ sim) :
-  ∀ p1 p2 (t1 : CTree' E R1) (t2 : CTree' E R2) (REFINE : RefineF φ sim p1 p2 t1 t2)
-    p1' p2',
-    RefineF φ sim p1' p2' t1 t2.
-Proof.
-  do 2 intro. revert p1.
-  induction p2 using (well_founded_induction olt_wf).
-  rename H into IHp2.
-  do 4 intro. revert IHp2.
-  induction REFINE.
-  - eauto.
-  - intros. econstructor 2; eauto.
-  - intros. econstructor 3; eauto.
-  - intros. econstructor 4; eauto.
-  - intros. econstructor 5; eauto.
-  - intros. eapply RefineF_contR; eauto.
-  Unshelve. all: exact None.
-Qed.
-
-Lemma BisimF_index_insensitive {R1 R2 E φ sim} (POSTFIX : sim <4= BisimF φ sim) :
-  ∀ p1 p2 (t1 : CTree' E R1) (t2 : CTree' E R2) (REFINE : BisimF φ sim p1 p2 t1 t2)
-    p1' p2',
-    BisimF φ sim p1' p2' t1 t2.
-Proof.
-  intros. destruct REFINE.
-  split; eapply RefineF_index_insensitive; eauto; intros; apply POSTFIX; auto.
-Qed.
-
-Definition Refine_index_insensitive {R1 R2 E} φ :
-  ∀ p1 p2 (t1 : CTree' E R1) (t2 : CTree' E R2) (REFINE : Refine φ p1 p2 t1 t2)
-    p1' p2',
-    Refine φ p1' p2' t1 t2.
-Proof.
-  pose proof (RefineF_index_insensitive (E := E) (Refine_postfix φ)).
-  intros. punfold REFINE. pfold.
-  eapply RefineF_monotone.
-  { eapply H. eapply RefineF_monotone; eauto. intros. pclearbot. auto. }
-  eauto.
-Qed.
-
-Definition Bisim_index_insensitive {R1 R2 E} φ :
-  ∀ p1 p2 (t1 : CTree' E R1) (t2 : CTree' E R2) (BISIM : Bisim φ p1 p2 t1 t2)
-    p1' p2',
-    Bisim φ p1' p2' t1 t2.
-Proof.
-  pose proof (BisimF_index_insensitive (E := E) (BisimF_postfix φ)).
-  intros. punfold BISIM. pfold.
-  eapply BisimF_monotone.
-  { eapply H. eapply BisimF_monotone; eauto. intros. pclearbot. auto. }
-  eauto.
-Qed.
-
 Lemma Refine_refl {R E} φ (R_REFL : ∀ v, φ v v) :
-  ∀ p1 p2 (t : CTree' E R), Refine φ p1 p2 t t.
+  ∀ t : CTree' E R, Refine φ t t.
 Proof.
   pcofix CIH.
-  intros. pfold. destruct t.
+  induction t; intros; pfold.
+  destruct t; try solve [destruct NCHOICE].
+  - econstructor 1; eauto.
   - econstructor 2; eauto.
   - econstructor 3; eauto.
-  - econstructor 4; eauto.
-  - econstructor 5; eauto. intros.
-    econstructor 6; eauto. instantiate (1 := c).
-    apply refine_prog with (p1' := Some 0) (p2' := Some 0); cbv; eauto.
-    all: instantiate (1 := None); simpl; auto.
-  Unshelve. all: exact None.
+  - econstructor 8; eauto.
+  - econstructor 4; eauto. intros. econstructor 5; eauto.
+    specialize (IHk c). punfold IHk.
 Qed.
 
 Lemma Bisim_refl {R E} φ (R_REFL : ∀ v, φ v v) :
-  ∀ p1 p2 (t : CTree' E R), Bisim φ p1 p2 t t.
+  ∀ t : CTree' E R, Bisim φ t t.
 Proof.
   pcofix CIH.
-  intros. pfold. destruct t.
+  induction t; intros; pfold.
+  destruct t; try solve [destruct NCHOICE].
+  - split; econstructor 1; eauto.
   - split; econstructor 2; eauto.
   - split; econstructor 3; eauto.
-  - split; econstructor 4; eauto.
-  - split; econstructor 5; eauto; intros;
-    econstructor 6; eauto; instantiate (1 := c);
-    apply refine_prog with (p1' := Some 0) (p2' := Some 0); cbv; eauto.
-    all: instantiate (1 := None); simpl; auto.
-  Unshelve. all: exact None.
+  - split; econstructor 8; eauto.
+  - split; econstructor 4; eauto; intros; econstructor 5; eauto.
+    all: specialize (IHk c); punfold IHk; apply IHk.
 Qed.
 
 Lemma Refine_inv_retL E R0 R1 R2
   (φ0 : R0 → R2 → Prop) (φ1 : R1 → R2 → Prop)
-  (sim0 : _ → _ → _ → _ → Prop)
-  (POSTFIX : sim0 <4= RefineF φ0 sim0)
-  (sim1 : _ → _ → _ → _ → Prop) :
-  ∀ p0' p1' t0 t1 (REFINE : RefineF (E := E) φ0 sim0 p0' p1' t0 t1) t0' r0 r1
+  (sim0 : _ → _ → Prop) (sim1 : _ → _  → Prop) :
+  ∀ t0 t1 (REFINE : RefineF (E := E) φ0 sim0 t0 t1) t0' r0 r1
     (IMPLφ : ∀ r2, φ0 r0 r2 → φ1 r1 r2)
-    (OBS0 : t0 = Ret r0) (OBS0' : t0' = Ret r1)
-    p0 p1,
-    RefineF (E := E) φ1 sim1 p0 p1 t0' t1.
+    (OBS0 : t0 = Ret r0) (OBS0' : t0' = Ret r1),
+    RefineF (E := E) φ1 sim1 t0' t1.
 Proof.
-  do 5 intro.
-  apply RefineF_index_insensitive with (p1' := Some 0) (p2' := p1') in REFINE; auto.
-  clear p0'. remember (Some 0) as p0' in REFINE. revert Heqp0'.
-  induction REFINE.
-  - intros; subst. cbv in LT1. destruct p1'; lia.
-  - inversion 3; subst. intros; subst.
-    econstructor 2; eauto.
-  - inversion 3.
-  - inversion 3.
-  - inversion 3.
-  - intros; subst. econstructor 6; eauto.
-  Unshelve. exact None.
+  induction 1.
+  - inversion 2; subst. intros; subst. econstructor 1; eauto.
+  - inversion 2.
+  - inversion 2.
+  - inversion 2.
+  - intros; subst. econstructor 5; eauto.
+  - inversion 2.
+  - intros; subst. econstructor 7; eauto.
+  - inversion 2.
 Qed.
 
 Lemma Refine_inv_retR E R0 R1 R2
   (φ0 : R0 → R1 → Prop) (φ1 : R0 → R2 → Prop)
-  (sim0 : _ → _ → _ → _ → Prop)
-  (POSTFIX : sim0 <4= RefineF φ0 sim0)
-  (sim1 : _ → _ → _ → _ → Prop) :
-  ∀ p0' p1' t0 t1 (REFINE : RefineF (E := E) φ0 sim0 p0' p1' t0 t1) t1' r1 r2
+  (sim0 : _ → _  → Prop) (sim1 : _ → _ → Prop) :
+  ∀ t0 t1 (REFINE : RefineF (E := E) φ0 sim0 t0 t1) t1' r1 r2
     (IMPLφ : ∀ r0, φ0 r0 r1 → φ1 r0 r2)
-    (OBS0 : t1 = Ret r1) (OBS0' : t1' = Ret r2)
-    p0 p1,
-    RefineF (E := E) φ1 sim1 p0 p1 t0 t1'.
+    (OBS0 : t1 = Ret r1) (OBS0' : t1' = Ret r2),
+    RefineF (E := E) φ1 sim1 t0 t1'.
 Proof.
-  do 5 intro.
-  apply RefineF_index_insensitive with (p1' := p0') (p2' := Some 0) in REFINE; auto.
-  clear p1'. remember (Some 0) as p1' in REFINE. revert Heqp1'.
-  induction REFINE.
-  - intros; subst. cbv in LT2. destruct p2'; lia.
-  - inversion 3; intros; subst.
-    econstructor 2; eauto.
-  - inversion 3.
+  induction 1.
+  - inversion 2; subst. intros; subst. econstructor 1; eauto.
+  - inversion 2.
+  - intros; econstructor 3; eauto.
   - intros; subst. econstructor 4; eauto.
-  - intros; subst. econstructor 5; eauto.
-  - inversion 3.
-  Unshelve. exact None.
+  - inversion 2.
+  - intros; subst. econstructor 6; eauto.
+  - inversion 2.
+  - inversion 2.
 Qed.
 
-Lemma Refine_inv_zeroR E R0 R1 R2 sim (sim' : _ → _ → _ → _ → Prop)
-  (φ : R0 → R1 → Prop) (φ' : R0 → R2 → Prop)
-  (POSTFIX : sim <4= RefineF φ sim) :
-  ∀ p0 p1 t0 t1 (REFINE : RefineF (E := E) φ sim p0 p1 t0 t1)
+Lemma Refine_inv_zeroR E R0 R1 R2 (sim : _ → _ → Prop) (sim' : _ → _ → Prop)
+  (φ : R0 → R1 → Prop) (φ' : R0 → R2 → Prop) :
+  ∀ t0 t1 (REFINE : RefineF (E := E) φ sim t0 t1)
     (OBS0 : t1 = Zero)
-    p0' p1' t1',
-    RefineF (E := E) φ' sim' p0' p1' t0 t1'.
+    t1',
+    RefineF (E := E) φ' sim' t0 t1'.
 Proof.
-  do 5 intro.
-  apply RefineF_index_insensitive with (p1' := p0) (p2' := Some 0) in REFINE; auto.
-  remember (Some 0) as p1' in REFINE.
-  revert Heqp1'. clear p1.
-  induction REFINE.
-  - intros; subst. cbv in LT2. destruct p2'; lia.
-  - inversion 2.
-  - inversion 2.
+  induction 1.
+  - inversion 1.
+  - inversion 1.
+  - intros; subst. econstructor 3; eauto.
   - intros; subst. econstructor 4; eauto.
-  - intros; subst. econstructor 5; eauto.
-  - inversion 2.
-  Unshelve. all:exact None.
+  - inversion 1.
+  - intros; subst. econstructor 6; eauto.
+  - inversion 1.
+  - inversion 1.
 Qed.
 
-Lemma Refine_inv_choiceL E R0 R1 sim (φ : R0 → R1 → Prop)
-  (POSTFIX : sim <4= RefineF φ sim) :
-  ∀ p0 p1 t0 t1 (REFINE : RefineF (E := E) φ sim p0 p1 t0 t1)
+Lemma Refine_inv_choiceL E R0 R1 (sim : _ → _ → Prop) (φ : R0 → R1 → Prop) :
+  ∀ t0 t1 (REFINE : RefineF (E := E) φ sim t0 t1)
     k (OBS0 : t0 = Choice k)
     c,
-    RefineF (E := E) φ sim p0 p1 (k c) t1.
+    RefineF (E := E) φ sim (k c) t1.
 Proof.
-  do 5 intro.
-  apply RefineF_index_insensitive with (p1' := Some 0) (p2' := p1) in REFINE; auto.
-  intros.
-  apply RefineF_index_insensitive with (p1 := Some 0) (p2 := p1); auto.
-  clear p0. revert p1 t0 t1 REFINE k OBS0 c.
-  remember (Some 0) as p0. do 4 intro. revert Heqp0.
-  induction REFINE.
-  - intros; subst. cbv in LT1. destruct p1'; lia.
-  - inversion 2.
-  - inversion 2.
-  - inversion 2.
-  - inversion 2; subst; clear_sig.
-    intros. eapply RefineF_index_insensitive; eauto.
-  - intros; subst.
-    exploit IHREFINE; eauto. instantiate (1 := c0).
-    intros.
-    econstructor 6; eauto.
+  induction 1.
+  - inversion 1.
+  - inversion 1.
+  - inversion 1.
+  - inversion 1; intros; subst. eauto.
+  - intros; subst. econstructor 5; eauto.
+  - inversion 1.
+  - intros; subst. econstructor 7; eauto.
+  - inversion 1.
 Qed.
 
-(*
-  RefineF φ sim p1 p2 t1 t2 ↔
-  ∀ p1' t1', t1 => t1' → ∃ p2' t2', t2 =>* t2' ∧ sim p1' p2' t1' t2'
-  and
-  ∀ p1' t1' ℓ, t1 =ℓ=> t1' → ∃ p2' t2', t2 =>*ℓ=>* t2' ∧ sim p1' p2' t1' t2'
-  and
-  ∀ r1, t1 ⇓ r1 → ∃ t2' r2, t2 =>* t2' ∧ t2' ⇓ r2 ∧ φ r1 r2
-*)
-
-(* RefineF φ12 sim12 p11 p12 t1 t2 *)
-(* RefineF φ23 sim23 p21 p22 t2 t3 *)
-(* does not imply RefineF (comp2 φ12 φ23) (comp4 sim12 sim23) p11 p22 t1 t3 *)
-(* this is because of the silent steps *)
-
-Lemma RefineF_transL {R1 R2 R3 E} (φ12 : R1 → R2 → Prop) (φ23 : R2 → R3 → Prop)
-  sim12 sim23
-  (POSTFIX12 : sim12 <4= RefineF (E := E) φ12 sim12)
-  (POSTFIX23 : sim23 <4= RefineF (E := E) φ23 sim23) :
-  ∀ p11 p12 t1 t2 (REFINE1 : RefineF (E := E) φ12 sim12 p11 p12 t1 t2)
-    p21 p22 t3 (REFINE2 : RefineF (E := E) φ23 sim23 p21 p22 t2 t3),
-    RefineF (comp2 φ12 φ23) (comp4 (RefineF φ12 sim12) sim23) p11 p22 t1 t3.
+Lemma Refine_inv_tauL E R0 R1 sim (φ : R0 → R1 → Prop)
+  (POSTFIX : sim <2= RefineF φ sim) :
+  ∀ t0 t1 (REFINE : RefineF (E := E) φ sim t0 t1)
+    t (OBS0 : t0 = Tau t),
+    RefineF (E := E) φ sim (obs_ctree t) t1.
 Proof.
-  do 5 intro. induction REFINE1.
-  - do 4 intro. apply POSTFIX12 in SIM. revert t1 SIM. induction REFINE2.
-    { intros. econstructor 1; cbv [comp4]; eauto. }
-    { intros.
-      eapply Refine_inv_retR; first [eassumption | reflexivity | idtac].
-      cbv [comp2]; eauto. }
-    { intros.
-      apply RefineF_index_insensitive with (p1' := Some 0) (p2' := Some 0) in SIM; auto.
-      remember (Some 0) as o' in SIM. revert Heqo'.
-      remember (Vis e k1) as t2 in SIM. revert Heqt2.
-      induction SIM.
-      { intros; subst. cbv in LT3. destruct p2'1; lia. }
-      { inversion 1. }
-      { inversion 1. intros; subst. clear_sig.
-        intros. econstructor 3; eauto. intros.
-        cbv [comp4]. exists p2'1, p1'0, (obs_ctree (k1 a)). eauto. }
-      { intros. subst. econstructor 4; eauto. }
-      { intros; subst. econstructor 5; eauto. }
-      { inversion 1. } }
-    { intros. eapply Refine_inv_zeroR; eauto. }
-    { intros.
-      apply RefineF_index_insensitive with (p1' := Some 0) (p2' := Some 0) in SIM; auto.
-      remember (Some 0) as o' in SIM. revert Heqo'.
-      remember (Choice k) as t2' in SIM. revert Heqt2'.
-      induction SIM.
-      { intros; subst. cbv in LT3. destruct p2'0; lia. }
-      { inversion 1. }
-      { inversion 1. }
-      { intros. subst. econstructor 4; eauto. }
-      { intros. subst. econstructor 5; eauto. }
-      { inversion 1; intros; subst. clear_sig. apply (IHk c).
-        eapply RefineF_index_insensitive; eauto. } }
-    { intros. econstructor 6; eauto. }
-  - intros; subst.
-    eapply Refine_inv_retL; first [eassumption | reflexivity | idtac].
-    cbv [comp2]. eauto.
-  - intros.
-    apply RefineF_index_insensitive with (p1' := Some 0) (p2' := p22) in REFINE2; auto.
-    remember (Some 0) as o' in REFINE2. revert Heqo'.
-    remember (Vis e k2) as t2 in REFINE2. revert Heqt2.
-    induction REFINE2.
-    { intros; subst. cbv in LT1. destruct p1'0; lia. }
-    { inversion 1. }
-    { inversion 1; subst; clear_sig.
-      intros; subst.
-      econstructor 3; eauto. intros.
-      specialize (CONT a). apply POSTFIX12 in CONT.
-      cbv [comp4]. eauto. }
-    { inversion 1. }
-    { inversion 1. }
-    { intros. econstructor 6; eauto. }
-  - intros. econstructor 4; eauto.
-  - intros. econstructor 5; eauto.
-  - intros. eapply IHREFINE1. eapply Refine_inv_choiceL in REFINE2; eauto.
+  induction 1.
+  - inversion 1.
+  - inversion 1.
+  - inversion 1.
+  - inversion 1.
+  - intros; subst. econstructor 5; eauto.
+  - inversion 1; intros; subst. eauto.
+  - intros; subst. econstructor 7; eauto.
+  - inversion 1; subst. econstructor 7; eauto.
 Qed.
 
-Lemma RefineF_transR {R1 R2 R3 E} (φ12 : R1 → R2 → Prop) (φ23 : R2 → R3 → Prop)
-  sim12 sim23
-  (POSTFIX12 : sim12 <4= RefineF (E := E) φ12 sim12)
-  (POSTFIX23 : sim23 <4= RefineF (E := E) φ23 sim23) :
-  ∀ p11 p12 t1 t2 (REFINE1 : RefineF (E := E) φ12 sim12 p11 p12 t1 t2)
-    p21 p22 t3 (REFINE2 : RefineF (E := E) φ23 sim23 p21 p22 t2 t3),
-    RefineF (comp2 φ12 φ23) (comp4 sim12 (RefineF φ23 sim23)) p11 p22 t1 t3.
+Lemma Refine_inv_tauR E R0 R1 sim (φ : R0 → R1 → Prop)
+  (POSTFIX : sim <2= RefineF φ sim) :
+  ∀ t0 t1 (REFINE : RefineF (E := E) φ sim t0 t1)
+    t (OBS1 : t1 = Tau t),
+    RefineF (E := E) φ sim t0 (obs_ctree t).
 Proof.
-  do 9 intro. revert p11 p12 t1 REFINE1. induction REFINE2.
-  - do 4 intro. apply POSTFIX23 in SIM. revert t2 SIM. induction REFINE1.
-    { intros. econstructor 1; cbv [comp4]; eauto. }
-    { intros. eapply Refine_inv_retL; eauto.
-      cbv [comp2]; eauto. }
-    { intros. clear LT1 LT2 p1 p3.
-      apply RefineF_index_insensitive with (p1' := Some 0) (p2' := Some 1) in SIM; auto.
-      remember (Some 0) as o' in SIM. revert Heqo'.
-      remember (Some 1) as o'' in SIM. clear Heqo''.
-      remember (Vis e k2) as t1 in SIM. revert Heqt1.
-      induction SIM.
-      { intros; subst. cbv in LT1. destruct p1'1; lia. }
-      { inversion 1. }
-      { inversion 1. intros; subst. clear_sig.
-        intros. econstructor 3; eauto. intros.
-        specialize (CONT0 a). apply POSTFIX23 in CONT0.
-        cbv [comp4]; eauto. }
-      { inversion 1. }
-      { inversion 1. }
-      { intros. subst. econstructor 6; eauto. } }
-    { intros. econstructor 4; eauto. }
-    { intros. econstructor 5; eauto. }
-    { intros. clear p3. rename p2'0 into p3.
-      apply IHREFINE1. eapply Refine_inv_choiceL; eauto. }
-  - intros; subst. eapply Refine_inv_retR; eauto.
-    cbv [comp2]. eauto.
-  - intros.
-    apply RefineF_index_insensitive with (p1' := p11) (p2' := Some 0) in REFINE1; auto.
-    remember (Some 0) as o' in REFINE1. revert Heqo'.
-    remember (Vis e k1) as t2 in REFINE1. revert Heqt2.
-    induction REFINE1.
-    { intros; subst. cbv in LT2. destruct p2'0; lia. }
-    { inversion 1. }
-    { inversion 1; subst; clear_sig.
-      intros; subst.
-      econstructor 3; eauto. intros.
-      specialize (CONT a). apply POSTFIX23 in CONT.
-      cbv [comp4]. eauto. }
-    { intros. econstructor 4; eauto. }
-    { intros. econstructor 5; eauto. }
-    { inversion 1. }
-  - intros. eapply Refine_inv_zeroR; eauto.
-  - intros.
-    apply RefineF_index_insensitive with (p1' := p11) (p2' := Some 0) in REFINE1; auto.
-    remember (Some 0) as o' in REFINE1. revert Heqo'.
-    remember (Choice k) as t2' in REFINE1. revert Heqt2'.
-    induction REFINE1.
-    { intros; subst. cbv in LT2. destruct p2'; lia. }
-    { inversion 1. }
-    { inversion 1. }
-    { intros; subst. econstructor 4; eauto. }
+  induction 1.
+  - inversion 1.
+  - inversion 1.
+  - intros. econstructor 3; eauto.
+  - intro; subst. econstructor 4; eauto.
+  - inversion 1.
+  - intros; subst. econstructor 6; eauto.
+  - inversion 1; subst. eauto.
+  - inversion 1; subst. econstructor 6; eauto.
+Qed.
+
+Lemma RefineF_trans {R1 R2 R3 E}
+  (φ12 : R1 → R2 → Prop) (φ23 : R2 → R3 → Prop) sim12 sim23
+  (POSTFIX12 : sim12 <2= RefineF (E := E) φ12 sim12)
+  (POSTFIX23 : sim23 <2= RefineF (E := E) φ23 sim23)
+  (TAUL : ∀ t1 t2, sim23 (Tau t1) t2 → sim23 (obs_ctree t1) t2)
+  (TAUR : ∀ t1 t2, sim23 t1 (Tau t2) → sim23 t1 (obs_ctree t2)) :
+  ∀ t1 t2 (REFINE1 : RefineF φ12 sim12 t1 t2)
+    t3 (REFINE2 : RefineF φ23 sim23 t2 t3),
+    RefineF (comp φ12 φ23) (comp sim12 sim23) t1 t3.
+Proof.
+  induction 1.
+  - intros. eapply Refine_inv_retL; eauto. cbv [comp]; eauto.
+  - intros. remember (Vis e k2) as t2 in REFINE2.
+    revert Heqt2. induction REFINE2; try solve [inversion 1].
+    { inversion 1; subst; clear_sig. econstructor 2; cbv [comp]; eauto. }
     { intros; subst. econstructor 5; eauto. }
-    { inversion 1; intros; subst; clear_sig. eauto. }
+    { intros; subst. econstructor 7; eauto. }
+  - intros. econstructor 3; eauto.
+  - intros. econstructor 4; eauto.
+  - intros. apply IHREFINE1. eapply Refine_inv_choiceL; eauto.
   - intros. econstructor 6; eauto.
-Qed.
+  - intros. apply IHREFINE1. eapply Refine_inv_tauL; eauto.
+  - intros. remember (Tau t2) as t2' in REFINE2.
+    revert Heqt2'. induction REFINE2; try solve [inversion 1].
+    { intros; subst. econstructor 5; eauto. }
+    { inversion 1; subst. admit. }
+    { intros; subst. econstructor 7; eauto. }
+    { inversion 1; subst. econstructor 8; cbv [comp]; eauto. }
+Abort.
 
-Lemma BisimF_trans_not_choice {R1 R2 R3 E}
-  (φ12 : R1 → R2 → Prop) (φ23 : R2 → R3 → Prop)
-  sim12 sim23
+Lemma RefineF_trans_tau {R1 R2 R3 E}
+  (φ12 : R1 → R2 → Prop) (φ23 : R2 → R3 → Prop) sim12 sim23
   (POSTFIX12 : sim12 <4= RefineF (E := E) φ12 sim12)
-  (POSTFIX23 : sim23 <4= RefineF (E := E) φ23 sim23) :
+  (POSTFIX23 : sim23 <4= RefineF (E := E) φ23 sim23)
+  (TAUL : ∀ p1 p2 t1 t2, sim23 p1 p2 (Tau t1) t2 → sim23 p1 p2 (obs_ctree t1) t2)
+  (TAUR : ∀ p1 p2 t1 t2, sim23 p1 p2 t1 (Tau t2) → sim23 p1 p2 t1 (obs_ctree t2)) :
   ∀ p11 p12 t1 t2 (REFINE1 : RefineF (E := E) φ12 sim12 p11 p12 t1 t2)
     p21 p22 t3 (REFINE2 : RefineF (E := E) φ23 sim23 p21 p22 t2 t3)
-    (NCHOICE : match t2 with Choice _ => False | _ => True end),
+    t (NOT : t2 = Tau t),
     RefineF (comp2 φ12 φ23) (comp4 sim12 sim23) p11 p22 t1 t3.
 Proof.
   do 9 intro. revert p11 p12 t1 REFINE1. induction REFINE2.
-  - do 4 intro. revert t2 SIM. induction REFINE1.
+  - do 4 intro. revert t2 SIM. induction REFINE1; try solve [inversion 2].
     { intros. econstructor 1; cbv [comp4]; eauto. }
+    { intros. econstructor 4; eauto. }
+    { intros. econstructor 5; eauto. }
+    { intros. econstructor 7; eauto. }
+    {  }
     { intros. eapply Refine_inv_retL; eauto.
       cbv [comp2]; eauto. }
     { intros. clear LT1 LT2 p1 p3. apply POSTFIX23 in SIM.
       apply RefineF_index_insensitive with (p1' := Some 0) (p2' := p2') in SIM; auto.
       remember (Some 0) as o' in SIM. revert Heqo'.
       remember (Vis e k2) as t1 in SIM. revert Heqt1.
-      induction SIM.
+      induction SIM; try solve [inversion 1].
       { intros; subst. cbv in LT1. destruct p1'1; lia. }
-      { inversion 1. }
       { inversion 1. intros; subst. clear_sig.
         intros. econstructor 3; eauto.
         cbv [comp4]; eauto. }
-      { inversion 1. }
-      { inversion 1. }
-      { intros. subst. econstructor 6; eauto. } }
+      { intros. subst. econstructor 6; eauto. }
+      { intros. subst. econstructor 8; eauto. } }
     { intros. econstructor 4; eauto. }
     { intros. econstructor 5; eauto. }
+    { destruct 2. }
+    { intros. econstructor 7; eauto. }
     { destruct 2. }
   - intros; subst. eapply Refine_inv_retR; eauto.
     cbv [comp2]. eauto.
@@ -649,18 +458,19 @@ Proof.
     apply RefineF_index_insensitive with (p1' := p11) (p2' := Some 0) in REFINE1; auto.
     remember (Some 0) as o' in REFINE1. revert Heqo'.
     remember (Vis e k1) as t2 in REFINE1. revert Heqt2.
-    induction REFINE1.
+    induction REFINE1; try solve [inversion 1].
     { intros; subst. cbv in LT2. destruct p2'0; lia. }
-    { inversion 1. }
     { inversion 1; subst; clear_sig.
       intros; subst.
       econstructor 3; cbv [comp4]; eauto. }
     { intros. econstructor 4; eauto. }
     { intros. econstructor 5; eauto. }
-    { inversion 1. }
+    { intros. econstructor 7; eauto. }
   - intros. eapply Refine_inv_zeroR; eauto.
   - destruct 2.
   - intros. econstructor 6; eauto.
+  - destruct 2.
+  - intros. econstructor 8; eauto.
 Qed.
 
 Lemma BisimF_trans {R1 R2 R3 E}
